
\begin{lem}[Amalgamation Lemma]
Let $A,B$ and $C$ in $\Klz$. If $A\dso B\dsu C$ % and $B\dsu C$ then
%Let $B=\gena{B_{1}}{C}$ and $B\dsu A$ then there exists a $D$ in
%$\Klf$ such that $C\dsu D$ and $A=\gena{A_{1}}{D}$.
then there exists $D\in\Klz$ as well as
Lie monomorphisms $\map{e}{A}{D}$ and $\map{f}{C}{D}$
such that
$A^{e}\dsu D$ and $C^{f}\dsu C$ and $B^{e}=B^{f}$ pointwise.
\end{lem}

\begin{proof}
Without loss of generality we can assume that $B\dsu A$ is a $\Klf$-minimal extension.

We first describe a \emph{na\"{i}ve amalgamation} {\bf (NAM)} that yields an $\nla{3}$-algebra
$D=
A\star_{B}C$ in which $A$ and $C$ embeds over $B$, moreover axiom $\sig{3}{2}$ will be shown to hold in $D$.

Secondly, a discussion on the different type of minimal extensions $A\quot B$
will provide axiom $\sig{3}{3}$ for $D$.

\begin{itemize}
\item[{\bf (NAM)}]
If we denote with $A^{\prime}$, $B^{\prime}$ and $C^{\prime}$, respectively $\tr{2}A$, $\tr{2}B$ and
$\tr{2}C$ then, after the definition of $\Klf$, we have $A^{\prime}\zso B^{\prime}\zsu C^{\prime}$.
We build the free $\nla{2}$-amalgam $D^{\prime}=\fram{A^{\prime}}{B^{\prime}}{C^{\prime}}$ of $A^{\prime}$ and $C^{\prime}$ over $B^{\prime}$. Assume $D^{\prime}$ is in $\Kl^{2}$ then, because
$B^{\prime}\zsu D^{\prime}$,
we $\delta_{2}$-strongly embed $D^{\prime}$ in $\K^{2}$ over $B^{\prime}$,
%we can find a copy of $D^{\prime}$ in 
we keep calling $D^{\prime}$ the isomorphic image in the generic model of $T^{2}$.

Consider $\ta D^{\prime}$ the $\ta$-closure of $D^{\prime}$ in $\K^{2}$,
because both $A^{\prime}$ and $C^{\prime}$ are selfsufficient in $D^{\prime}$
and $D^{\prime}\zsu\ta D^{\prime}$, we have that $A^{\prime}$ and $C^{\prime}$ are both $\delta_{2}$-strong
in $\ta D^{\prime}$. Moreover $\ta$-closure implies
\begin{labeq}{inter}
B^{\prime}=\gena{B_{1}}{\ta D^{\prime}}=\gena{\abu}{\ta D^{\prime}}\cap\gena{\cbu}{\ta D^{\prime}}.
\end{labeq}

Now on account of Lemma \ref{bellemma},
there exist two embeddings $j_{A}$ and $j_{C}$ of $\fr{3}\tr{2}A$ and $\fr{3}\tr{2}C$
into $\fr{3}\ta D^{\prime}$ their images being $\gena{\abu}{\fr{3}\ta D^{\prime}}$ and $\gena{\cbu}
{\fr{3}\ta D^{\prime}}$ respectively. From \pref{inter} and lemma \ref{bellemmino} instead, we get
\begin{labeq}{freeint}
\gena{B_{1}}{\fr{3}\ta D^{\prime}}=\gena{\abu}{\fr{3}\ta D^{\prime}}\cap\gena{\cbu}{\fr{3}\ta D^{\prime}}
\end{labeq}
here $B_{1}$, $\abu$ and $\cbu$ are identified with its images modulo $j_{A}$ and $j_{C}$. 

We set $N^{3}(A)^{\bullet}=j_{A}(N^{3}(A))$ and $N^{3}(C)^{\bullet}=j_{C}(N^{3}(C))$.
And we build
$$D=\fr{3}\ta D^{\prime}\quot(N^{3}(A)^{\bullet}+N^{3}(C)^{\bullet}).$$
As $N^{3}(A)^{\bullet}+N^{3}(C)^{\bullet}$ is an ideal consisting only of weight $3$ elements,
$\fr{3}\tr{2}D=\fr{3}(\tr{2}\fr{3}\ta D^{\prime})%\simeq
=\fr{3}\ta D^{\prime}$, hence we obtain $N^{3}(D)=N^{3}(A)^{\bullet}+N^{3}(C)^{\bullet}$.

From \pref{freeint} we have that
$$N^{3}(B)^{\bullet}:=j_{A}(N^{3}(B))=N^{3}(A)^{\bullet}\cap N^{3}(C)^{\bullet}=j_{C}(N^{3}(B))$$
and the following compatibility equations
\begin{labeq}{compa}
N^{3}(A)^{\bullet}=N^{3}(D)\cap\gena{\abu}{\fr{3}\ta D^{\prime}}
\end{labeq}and
$$
N^{3}(C)^{\bullet}=N^{3}(D)\cap\gena{\cbu}{\fr{3}\ta D^{\prime}}.
$$

So far, are $A$ and $C$ embeddable in $D$ via Lie Algebra monomorphisms,
just regard $A\simeq\fr{3}\tr{2}A\quot N^{3}(A)$ and take the quotient of $j_{A}$:
\begin{eqnarray}
\map{\bar j _{A}}{&\fr{3}\tr{2}A\quot N^{3}(A)}{D}\\
&\bar w\longmapsto \bar w
\end{eqnarray}
on account of \pref{compa} is $\bar j_{A}$ one-to-one, in particular its image is again
$\gena{\abu}{D}=(\gena{\abu}{\fr{3}\ta D^{\prime}}+N^{3}(D))\quot N^{3}(D)$.\quad Do the same for $C$.

\medskip
We show next that if $B_{1}\dsu A_{1}$ then the embedding of $C$ into $D$ is $\delta_{3}$-strong.
We have to prove $\delta_{3}E_{1}\geq\delta_{3}C_{1}$ for each $E_{1}\zsu\ta D_{1}$ such that
$E_{1}\nni\cbu$ and $E_{1}$ $\ta$-closed.

We first observe $\delta_{3}E_{1}\geq\delta_{3} E_{1}\cap D_{1}$. This is because $d_{2}E_{1}\geq
d_{2}E_{1}\cap D_{1}$ and
\begin{multline}\label{ntreonto}
N^{3}(E_{1})=\\
=N^{3}(D)\cap\gena{E_{1}}{\fr{3}\ta D^{\prime}}=
(N^{3}(A)+N^{3}(C))\cap\gena{E_{1}}{\fr{3}\ta D^{\prime}}=\\
=(N^{3}(A)\cap\gena{E_{1}}{\fr{3}\ta D^{\prime}})+N^{3}(C)=\\
=(N^{3}(D)\cap\gena{A_{1}}{\fr{3}\ta D^{\prime}}\cap\gena{E_{1}}{\fr{3}\ta D^{\prime}})+N^{3}(C)=\\
=(N^{3}(D)\cap\gena{A_{1}\cap E_{1}}{\fr{3}\ta D^{\prime}})+N^{3}(C)\inn\\
\inn N^{3}(E_{1}\cap A_{1}+C_{1})\inn N^{3}(E_{1}\cap D_{1})
\end{multline}
Therefore we have to show $\delta_{3}E_{1}\cap D_{1}\geq\delta_{3}C_{1}$.

As $E_{1}\cap D_{1}=C_{1}+(E_{1}\cap \abu)$ we finish once we show
$\delta_{3}(E_{1}\cap D_{1}\quot C)=\delta_{3}(E_{1}\cap\abu\quot B)$ because
%$E_{1}\cap \abu$ is a $\delta_{2}$ strong subspace of $\abu$ and 
$B\dsu A$ and $\delta_{3}(E_{1}\cap \abu\quot B)\geq 0$.

We have
%$$\delta_{3}(E_{1}\cap D_{1}\quot C)
$$\delta_{3}(E_{1}\cap D_{1})-\delta_{3}(C_{1})=
d_{2}(E_{1}\cap D_{1}\quot C_{1})
-\big(\dfp(N^{3}(E_{1}\cap D_{1}))-\dfp(N^{3}(C))\big).$$
Everything behaves good for $d_{2}$, we have $d_{2}(E_{1}\cap D_{1})-d_{2}(C_{1})=
d_{2}(E_{1}\cap\abu)-d_{2}B_{1}$. (\dots eigentlich stimmt das f`\"ur $\delta_{2}$ aber
man kann approximieren \dots)

To conclude we have to show
$$N^{3}(E_{1}\cap\abu)\quot N^{3}(B)^{\bullet}\simeq
N^{3}(C_{1}+(E_{1}\cap \abu))\quot N^{3}(C)^{\bullet}.$$
Consider the map
\begin{eqnarray*}
N^{3}(E_{1}\cap \abu)\quot N^{3}(B)^{\bullet}&\longrightarrow&N^{3}(E_{1}\cap D_{1})\quot N^{3}(C)^{\bullet}\\
\bar\eta&\longmapsto&\bar\eta\quad\quad\forall\eta\in N^{3}(E_{1}\cap\abu).
\end{eqnarray*}
Soundness is immediate. Moreover our map is injective because
\begin{multline*}
N^{3}(C)^{\bullet}\cap\gena{E_{1}\cap \abu}{\fr{3}\ta D^{\prime}}=\\
=N^{3}(D)\cap\gena{\cbu}{\fr{3}\ta D^{\prime}}\cap\gena{E_{1}\cap \abu}{\fr{3}\ta D^{\prime}}=\\
=N^{3}(D)\cap\gena{\abu\cap C_{1}}{\fr{3}\ta D^{\prime}}=N^{3}(B)^{\bullet}.
\end{multline*}
Here we used $\gena{\cbu}{\fr{3}\ta D^{\prime}}\cap\gena{E_{1}\cap\abu}{\fr{3}\ta D^{\prime}}=
\gena{\cbu\cap\abu}{\fr{3}\ta D^{\prime}}$ because both $\cbu$ and $E_{1}\cap\abu$ are $\delta_{2}$ strong in $D_{1}$ and $\ta$ closed and because $\gena{\cbu}{\ta D^{\prime}}\cap\gena{E_{1}\cap\abu}{\ta D^{\prime}}=\gena{\bbu}{\ta D^{\prime}}$.

To see that this map is onto use the arguments in \pref{ntreonto} again to get
$$N^{3}(E_{1}\cap D_{1})=(
N^{3}(D)\cap\gena{E_{1}\cap A_{1}}{\fr{3}\ta D^{\prime}})+N^{3}(C)^{\bullet}.$$
%On the other hand, since again $\gena{\abu}{\ta D^{\prime}}\cap\gena{E_{1}}{\ta D^{\prime}}=\gena{E_{1}\cap\abu}{\ta D^{\prime}}$ we have
%\begin{multline*}
%N^{3}(E_{1})=N^{3}(D)\cap\gena{E_{1}}{\fr{3}\ta D^{\prime}}=\\
%=(N^{3}(A)^{\bullet}+N^{3}(C)^{\bullet})\cap\gena{E_{1}}{\fr{3}\ta D^{\prime}}=\\
%=(N^{3}(A)^{\bullet}\cap\gena{E_{1}}{\fr{3}\ta D^{\prime}})+N^{3}(C)^{\bullet}=\\
%=(N^{3}(D)\cap\gena{E_{1}\cap A_{1}}{\fr{3}\ta D^{\prime}})+N^{3}(C)^{\bullet}
%\end{multline*}
%and this gives that our map is onto.

We have shown that
$$\dfp(N^{3}(E))-\dfp(N^{3}(C))=\dfp(N^{3}(E_{1}\cap\abu))-\dfp(N^{3}(B)^{\bullet})$$
thus $C$ is $\delta_{3}$-strong embeddable in $D$.

A completely analogous argument proves that $A$ is $\delta_{3}$-strong in $D$.
\end{itemize}

\smallskip
We show that $D$ has $\sig{3}{2}$.
It suffices to show $\delta_{3}H_{1}\geq2$ for each  $H_{1}\zsu\ta D_{1}$ of finite linear dimension. 

Consider the relative $\ta$-closure $H_{1}^{+}$ of $H_{1}$ in $D$, then it holds
$\gena{H_{1}^{+}}{\tr{2}D}\cap\gena{C_{1}}{\tr{2}D}=\gena{H_{1}^{+}\cap C_{1}}{\tr{2}D}$.

By lemma \ref{}, since $C_{1}\dsu\ta D_{1}$, we have
$$
\delta_{3}(H_{1}^{+}+C_{1})+\delta_{3}(H_{1}^{+}\cap C_{1})
\leq\delta_{3}H_{1}^{+}+\delta_{3}C_{1}\leq\delta_{3}H_{1}^{+}+\delta_{3}(H_{1}^{+}+C_{1}).
$$
Now as $C\in\Klf$, we conclude
$\delta_{3}H_{1}\geq\delta_{3}H_{1}^{+}\geq\delta_{3}(H_{1}^{+}\cap C_{1})\geq2$.


To conclude the proof we have to
show that $\tr{2}D$ actually lies in $\Kl^{2}$ and provide axiom $\sig{3}{2}$ for $D$.
\end{proof}
